tests/vfmTestLib.sml
@@ -49,8 +49,7 @@ val cv_eval_run_block_rwts = [
 
 fun trim2 s = Substring.string(Substring.triml 2 (Substring.full s))
 
-(* TODO: build the actual domain from the test *)
-val empty_accs_str = "NONE"
+val empty_accs_str = "(Collect empty_domain)"
 
 fun mk_statement isHash test_name prev_hashes =
   if isHash then
